DumbContracts/Examples/Counter.lean
@@ -46,6 +46,7 @@ def exampleUsage : Contract Uint256 := do
   storage := fun _ => 0,
   storageAddr := fun _ => "",
   storageMap := fun _ _ => 0,
+  storageMapAddr := fun _ _ => "",
   sender := "0xAlice",
   thisAddress := "0xCounter",
   msgValue := 0,
