DumbContracts/Proofs/SimpleToken/Basic.lean
@@ -150,6 +150,7 @@ private theorem mint_unfold (s : ContractState) (to : Address) (amount : Uint256
       storageMap := fun slot addr =>
         if (slot == 1 && addr == to) = true then EVM.Uint256.add (s.storageMap 1 to) amount
         else s.storageMap slot addr,
+      storageMapAddr := s.storageMapAddr,
       sender := s.sender,
       thisAddress := s.thisAddress,
       msgValue := s.msgValue,
@@ -218,6 +219,7 @@ private theorem transfer_unfold (s : ContractState) (to : Address) (amount : Uin
         if (slot == 1 && addr == to) = true then EVM.Uint256.add (s.storageMap 1 to) amount
         else if (slot == 1 && addr == s.sender) = true then EVM.Uint256.sub (s.storageMap 1 s.sender) amount
         else s.storageMap slot addr,
+      storageMapAddr := s.storageMapAddr,
       sender := s.sender,
       thisAddress := s.thisAddress,
       msgValue := s.msgValue,
